CODIGO/GRAFOS/Auxiliar/Graph.dfy
@@ -6,7 +6,7 @@ type Graph = (set<Node>, set<Edge>)
 
 function invert (graph:Graph) : (r:Graph)
 requires isValidGraph(graph)
-ensures isValidGraph(r)
+ensures isValidGraph(r) 
 {
     var allEdges:set<Edge> := (set n1,n2 | n1 in graph.0 && n2 in graph.0 && n1 != n2 :: {n1,n2});
     var invertGraph:Graph := (graph.0, allEdges-graph.1);
