CODIGO/GRAFOS/Transformations/CliqueToIndependentSet.dfy
@@ -4,6 +4,7 @@ include "../Problems/IndependentSet.dfy"
 
 function Clique_to_IndependentSet(graph:Graph, k:int) : (r:(Graph,int))
     requires isValidGraph(graph)
+    ensures isValidGraph(r.0)
 {
     (invert(graph),k)
 }
@@ -24,7 +25,7 @@ lemma Clique_IndependentSet1(graph:Graph, k:int)
 {   
     var (Vgraph,Vk) := Clique_to_IndependentSet(graph,k);
     if (IndependentSet(Vgraph,Vk)) {
-        var IndepSet:set<Node> :| isIndependentSet(IndepSet,Vgraph.1) && |IndepSet| >= Vk && IndepSet <= Vgraph.0;
+        var IndepSet:set<Node> :| IndepSet <= Vgraph.0 && isIndependentSet(IndepSet,Vgraph) && |IndepSet| >= Vk;
 
         var clique:set<Node> := IndepSet;
 
@@ -32,7 +33,7 @@ lemma Clique_IndependentSet1(graph:Graph, k:int)
         auxIndependentSet(IndepSet,Vgraph);
         assert forall u,v | u in IndepSet && v in IndepSet && u != v :: {u,v} !in Vgraph.1;
 
-        assert isClique(clique,graph.1) && |clique| >= k && clique <= graph.0;
+        assert isClique(clique,graph) && |clique| >= k && clique <= graph.0;
     }
 }
 
@@ -43,13 +44,13 @@ lemma Clique_IndependentSet2(graph:Graph, k:int)
 {
     if (Clique(graph,k)) {
         var (Vgraph,Vk) := Clique_to_IndependentSet(graph,k);
-        var clique:set<Node> :| isClique(clique,graph.1) && |clique| >= k && clique <= graph.0;
+        var clique:set<Node> :| clique <= graph.0 && isClique(clique,graph) && |clique| >= k;
 
         var IndepSet:set<Node> := clique;
 
         // Demostracion 1 : isIndependentSet(IndepSet,graph.1)
         auxIndependentSet(IndepSet,Vgraph);
 
-        assert isIndependentSet(IndepSet,Vgraph.1) && |IndepSet| >= Vk && IndepSet <= Vgraph.0;
+        assert isIndependentSet(IndepSet,Vgraph) && |IndepSet| >= Vk && IndepSet <= Vgraph.0;
     }
 }
