CODIGO/SUMA/Transformations/ParticionIntToSumaInt.dfy
@@ -48,26 +48,15 @@ lemma ParticionInt_Suma2(A:multiset<int>)
           ParticionInt(A) ==> SumaInt(SA,SS)
 {
     // A = {1, 2, 3}
+    var (SA,SS) := ParticionInt_to_SumaInt(A);
     if (ParticionInt(A)) {
-        if (GSumInt(A) % 2 == 1) {
-            var (SA,SS) := ParticionInt_to_SumaInt(A);
-            var S:multiset<int> := multiset{};
-            assume S <= SA && GSumInt(S) == SS;
-        }
-        else {
-            var (SA,SS) := ParticionInt_to_SumaInt(A);
             var P1:multiset<int>, P2:multiset<int> :| P1 <= A && P2 <= A && P1 + P2 == A && GSumInt(P1) == GSumInt(P2); // {1,2} {3}
-
+            GSumIntPartes(A,P1,P2);
+            assert GSumInt(A) == 2 * GSumInt(P1);
+            FSumIntComputaGSumInt(A);
+            assert FSumInt(A) % 2 == 0;
+             
             var S:multiset<int> := P1;
-
-            assume A == SA;
-            
-            //Demostracion 2: GSumInt(S) == SS
-            FSumIntComputaGSumInt(S); FSumIntComputaGSumInt(A);
-            assert GSumInt(A)/2 == SS;
-            assume GSumInt(P1) == SS;
-
             assert S <= SA && GSumInt(S) == SS;
-        }
     }
 }
